lawyer/nonblocking/mk_ref_adequacy.v
@@ -1,0 +1,11 @@
+From lawyer.nonblocking Require Import mk_ref wfree_adequacy.
+
+Theorem mk_ref_is_wait_free: wait_free mk_ref (fun _ => True).
+Proof using.
+  pose proof (wfree_is_wait_free _ mk_ref_WF_spec).
+  simpl in H.
+  (* TODO: make init st condition transparent *)
+  admit.
+Admitted. 
+
+Print Assumptions mk_ref_is_wait_free. 
